Change lattice (remove bottom as Hack/Seidel/Willhelm propose).

ConstantPropagation.v
@@ -1,8 +1,7 @@
-
 Require Import CSet Le.
 
 Require Import Plus Util AllInRel Map.
-Require Import CSet Val Var Env EnvTy IL Sim SimApx Fresh Annotation MoreExp Coherence.
+Require Import CSet Val Var Env EnvTy IL Sim Fresh Annotation MoreExp Coherence LabelsDefined.
 
 Require Import Liveness Filter SetOperations ValueOpts.
 
@@ -13,70 +12,51 @@ Unset Printing Records.
 
 
 (* None is top *)
-Definition aval := option val.
-
-
-
-Definition binop_eval (o:binop) (v1 v2:aval) : option aval :=
-  match v1, v2 with
-    | Some v1, Some v2 =>
-      match Exp.binop_eval o v1 v2 with
-        | None => None (* if binop_eval says None, it's undefined, so we yield bottom, not top *)
-        | Some x => Some (Some x)
-      end
-      | _, _  => Some None (* if v1 or v2 is top, we yield top *)
-  end.
+Definition aval := val.
 
 Fixpoint exp_eval (E:onv aval) (e:exp) : option aval :=
   match e with
-    | Con v => Some (Some v)
+    | Con v => Some v
     | Var x => E x
     | BinOp o e1 e2 => mdo v1 <- exp_eval E e1;
                       mdo v2 <- exp_eval E e2;
-                      binop_eval o v1 v2
+                      Exp.binop_eval o v1 v2
   end.
 
-Inductive le : option aval -> option aval -> Prop :=
-  | leTop x : le x (Some None)
-  | leValVal y : le (Some (Some y)) (Some (Some y))
-  | leBotBot y : le None (Some (Some y))
-  | leBot  : le None None.
+Inductive le_precise : option aval -> option aval -> Prop :=
+  | leTop x : le_precise None x
+  | leValVal y : le_precise (Some y) (Some y)
+  | leBot  : le_precise None None.
 
 
 
-Inductive cp_sound : list (params*list (option aval))
+Inductive cp_sound (AE:onv aval) : list (params)
                       -> stmt
-                      -> ann (onv aval)
-                      -> ann (set var)
                       -> Prop :=
-| CPOpr (x:var) Cp b e (Gamma:onv aval) al lv alv
-  : cp_sound Cp b al alv
-    -> agree_on eq (getAnn alv \ {{x}}) Gamma (getAnn al)
-    -> exp_eval Gamma e = getAnn al x
-    -> cp_sound Cp (stmtExp x e b) (ann1 Gamma al) (ann1 lv alv)
-| CPIf Cp e b1 b2 Gamma lv al1 al2 alv1 alv2
-  : agree_on eq lv Gamma (getAnn al1)
-    -> agree_on eq lv Gamma (getAnn al2)
-    (* these conditions make it conditional constant propagation *)
-    -> (exp_eval Gamma e <> Some (Some 1) -> cp_sound Cp b1 al1 alv1)
-    -> (exp_eval Gamma e <> Some (Some 0) -> cp_sound Cp b2 al2 alv2)
-    -> cp_sound Cp (stmtIf e b1 b2) (ann2 Gamma al1 al2) (ann2 lv alv1 alv2)
-| CPGoto l Y Cp Gamma lv Z Yf
-  : get Cp (counted l) (Z,Yf)
-    -> PIR2 le (List.map (exp_eval Gamma) Y) Yf
-    -> cp_sound Cp (stmtGoto l Y) (ann0 Gamma) (ann0 lv)
-| CPReturn Cp e  Gamma lv
-  : cp_sound Cp (stmtReturn e) (ann0 Gamma) (ann0 lv)
-| CPLet Cp s Z b Gamma lv Yf als alb alvs alvb
-  : cp_sound ((Z,Yf)::Cp) s als alvs
-  -> cp_sound ((Z,Yf)::Cp) b alb alvb
-  -> agree_on eq lv (Gamma[Z <-- Yf]) (getAnn als)
-  -> agree_on eq lv Gamma (getAnn alb)
-  -> cp_sound Cp (stmtLet Z s b) (ann2 Gamma als alb) (ann2 lv alvs alvb).
+| CPOpr (x:var) Cp b e
+  : cp_sound AE Cp b
+    -> exp_eval AE e = AE x
+    -> cp_sound AE Cp (stmtExp x e b)
+| CPIf Cp e b1 b2
+  : (* these conditions make it conditional constant propagation *)
+    (exp_eval AE e <> (Some val_false) -> cp_sound AE Cp b1)
+    -> (exp_eval AE e <> (Some val_true) -> cp_sound AE Cp b2)
+    -> cp_sound AE Cp (stmtIf e b1 b2)
+| CPGoto l Y Cp Z
+  : get Cp (counted l) Z
+    -> length Z = length Y
+    -> PIR2 le_precise (lookup_list AE Z) (List.map (exp_eval AE) Y)
+    -> cp_sound AE Cp (stmtGoto l Y)
+| CPReturn Cp e
+  : cp_sound AE Cp (stmtReturn e)
+| CPLet Cp s Z b
+  : cp_sound AE (Z::Cp) s
+  -> cp_sound AE (Z::Cp) b
+  -> cp_sound AE Cp (stmtLet Z s b).
 
 Definition cp_eqn E x :=
   match E x with
-    | Some (Some c) => {{(Var x, Con c)}}
+    | Some c => {{(Var x, Con c)}}
     | _ => ∅
   end.
 
@@ -113,18 +93,11 @@ Proof.
   intuition.
 Qed.
 
-Instance entails_refl
-: Reflexive (entails).
-Proof.
-  hnf; intros. unfold entails; intros; split; eauto; try reflexivity.
-Qed.
-
 Lemma entails_monotonic_add Gamma Γ' gamma
 : entails Gamma Γ' -> entails (gamma ∪ Gamma) Γ'.
 Proof.
-  unfold entails; intros; dcr; split.
-  - intros. eapply H0. hnf; intros. eapply H; eauto. cset_tac; intuition.
-  - rewrite H1. rewrite eqns_freeVars_union. cset_tac; intuition.
+  unfold entails; intros; dcr.
+  - hnf; intros. eapply H. hnf; intros. eapply H0. cset_tac; intuition. eauto.
 Qed.
 
 Lemma map_agree X `{OrderedType X} Y `{OrderedType Y}
@@ -188,46 +161,24 @@ Definition cp_eqns_ann (a:ann (onv aval)) (b:ann (set var)) : ann eqns :=
 
 Definition cp_choose_exp E e :=
   match exp_eval E e with
-    | Some (Some c) => Con c
+    | Some c => Con c
     | _ => e
   end.
 
 
-Fixpoint cp_choose s (a:ann (onv aval)) : ann args :=
-  match s, a with
-    | stmtExp x e s, ann1 E an =>
-      ann1 (cp_choose_exp E e::nil) (cp_choose s an)
-    | stmtIf e s t, ann2 E ans ant =>
-        ann2 (cp_choose_exp E e::nil) (cp_choose s ans) (cp_choose t ant)
-    | stmtGoto f Y, ann0 E =>
-      ann0 (List.map (cp_choose_exp E) Y)
-    | stmtReturn e, ann0 E => ann0 (cp_choose_exp E e::nil)
-    | stmtLet Z s t, ann2 E ans ant =>
-      ann2 nil (cp_choose s ans) (cp_choose t ant)
-    | _, _ => ann0 nil
+Fixpoint cp_choose (AE:onv aval) s : ann args :=
+  match s with
+    | stmtExp x e s =>
+      ann1 (cp_choose_exp AE e::nil) (cp_choose AE s)
+    | stmtIf e s t =>
+        ann2 (cp_choose_exp AE e::nil) (cp_choose AE s) (cp_choose AE t)
+    | stmtGoto f Y =>
+      ann0 (List.map (cp_choose_exp AE) Y)
+    | stmtReturn e => ann0 (cp_choose_exp AE e::nil)
+    | stmtLet Z s t =>
+      ann2 nil (cp_choose AE s) (cp_choose AE t)
+    | _ => ann0 nil
   end.
-
-Lemma exp_eval_moreDefined e lv Gamma v
-: (forall x v, Gamma x = Some (Some v) -> moreDefined (cp_eqns Gamma lv) (cp_eqns Gamma lv) (Var x) (Con v))
-  -> live_exp_sound e lv
-   -> exp_eval Gamma e = ⎣⎣v ⎦ ⎦
-   -> moreDefined (cp_eqns Gamma lv) (cp_eqns Gamma lv) e (Con v).
-Proof.
-  intros. general induction H0; simpl in * |- *; hnf; intros; simpl; eauto using fstNoneOrR.
-  - econstructor; eauto.
-  - eapply H0; eauto.
-  - monad_inv H1.
-    destruct x, x0; isabsurd.
-    exploit IHlive_exp_sound1; eauto.
-    exploit IHlive_exp_sound2; eauto.
-    exploit X; try eapply H0; eauto. exploit X0; try eapply H0; eauto.
-    simpl in * |- *. inv X1; inv X2; simpl.
-    + econstructor.
-    + econstructor.
-    + econstructor.
-    + destruct (Exp.binop_eval o v0 v1). inv EQ2. econstructor. eauto.
-      congruence.
-Qed.
 
 Lemma zip2Ann_get X Y Z (f:X->Y->Z) a b z
 :
@@ -254,10 +205,8 @@ Lemma entails_union_split Gamma Γ' Γ''
 Proof.
   unfold entails, satisfiesAll.
   split; intros; dcr.
-    + split; intros. eapply H0; eauto. cset_tac; intuition.
-      rewrite <- H1. rewrite eqns_freeVars_union. eapply incl_left.
-    + split; intros. eapply H0; eauto. cset_tac; intuition.
-      rewrite <- H1. rewrite eqns_freeVars_union. eapply incl_right.
+    + eapply H; eauto. cset_tac; intuition.
+    + eapply H; eauto. cset_tac; intuition.
 Qed.
 
 Lemma entails_union Gamma Γ' Γ''
@@ -266,9 +215,8 @@ Lemma entails_union Gamma Γ' Γ''
 -> entails Gamma (Γ' ∪ Γ'').
 Proof.
   unfold entails, satisfiesAll.
-  split; intros; dcr.
+  intros; dcr.
   + intros. cset_tac. destruct H1; eauto.
-  + rewrite eqns_freeVars_union. cset_tac; intuition.
 Qed.
 
 Instance option_R_trans `{Transitive} : Transitive (option_R R).
@@ -276,9 +224,9 @@ Proof.
   hnf; intros. inv H0; inv H1. econstructor; eauto.
 Qed.
 
-Lemma cp_eqns_in AE x lv v
+Lemma in_cp_eqns AE x lv v
   : x \In lv
-    -> AE x = ⎣⎣v ⎦ ⎦
+    -> AE x = ⎣v ⎦
     -> (Var x, Con v) ∈ cp_eqns AE lv.
 Proof.
   intros. unfold cp_eqns.
@@ -292,134 +240,308 @@ Qed.
 
 Lemma cp_eqns_satisfies_env AE E x v lv
 : x ∈ lv
-  -> AE x = ⎣⎣v ⎦ ⎦
+  -> AE x = ⎣v ⎦
   -> satisfiesAll E (cp_eqns AE lv)
   -> E x = ⎣v ⎦.
 Proof.
   intros. exploit H1; eauto.
   instantiate (1:=(Var x, Con v)).
-  eapply cp_eqns_in; eauto.
+  eapply in_cp_eqns; eauto.
   hnf in X; simpl in *. inv X; eauto.
 Qed.
 
-Lemma exp_eval_same e lv AE E v v'
-:   live_exp_sound e lv
-    -> exp_eval AE e = ⎣⎣v ⎦ ⎦
+Lemma exp_eval_same e lv AE E v
+:   Exp.freeVars e ⊆ lv
+    -> exp_eval AE e = ⎣v ⎦
     -> satisfiesAll E (cp_eqns AE lv)
-    -> Exp.exp_eval E e = Some v'
-    -> option_R eq ⎣v' ⎦ ⎣v ⎦.
+    -> exists v', Exp.exp_eval E e = Some v' /\ option_eq eq ⎣v' ⎦ ⎣v ⎦.
 Proof.
-  intros. general induction H; simpl in * |- *; eauto using option_R.
+  intros. general induction e; simpl in * |- *; eauto 20 using @option_eq.
   - exploit cp_eqns_satisfies_env; eauto.
-    rewrite X; eauto using option_R.
-  - monad_inv H1. monad_inv H3.
-    destruct x, x0; isabsurd.
-    exploit IHlive_exp_sound1; eauto.
-    exploit IHlive_exp_sound2; eauto.
-    rewrite EQ0, EQ4; simpl. rewrite EQ5.
-    inv X. inv X0. simpl in *. rewrite EQ5 in EQ2.
-    inv EQ2. constructor; eauto.
+    + rewrite <- H. cset_tac; eauto.
+    + rewrite H0.
+      eexists v0; split; eauto using @option_eq.
+  - monad_inv H0.
+    edestruct IHe1; eauto. cset_tac; intuition.
+    edestruct IHe2; eauto. cset_tac; intuition.
+    dcr.
+    rewrite H3, H2, EQ, EQ1; simpl.
+    inv H4; inv H5.
+    rewrite EQ2.
+    eexists v; split; eauto using @option_eq.
 Qed.
 
 Lemma exp_eval_entails AE e v x lv
-: live_exp_sound e lv
-  -> exp_eval AE e = ⎣⎣v ⎦ ⎦
+: Exp.freeVars e ⊆ lv
+  -> exp_eval AE e = ⎣v ⎦
   -> entails ({{ (Var x, e) }} ∪ cp_eqns AE lv) {{(Var x, Con v)}}.
 Proof.
   intros.
-  unfold entails; split; intros. unfold satisfiesAll, satisfies; intros.
+  unfold entails; intros. unfold satisfiesAll, satisfies; intros.
   exploit (H1 (Var x, e)); eauto.
   cset_tac; intuition. cset_tac. invc H2; simpl in *; subst; simpl.
-  inv X.
   eapply satisfiesAll_union in H1; dcr.
-  exploit exp_eval_same; try eapply H1; eauto.
-  etransitivity. instantiate (1:=(eqns_freeVars {{(Var x, e)}})).
-  unfold eqns_freeVars.
-  repeat rewrite map_single; eauto using freeVars_Proper.
-  repeat rewrite (@fold_single _ _ _ Equal).
-  simpl. cset_tac; intuition.
-  eapply Equal_ST. eapply union_m. eapply transpose_union.
-  eapply Equal_ST. eapply union_m. eapply transpose_union.
-  assert ( {(Var x, e); {}} ⊆ {(Var x, e); {}} ∪ cp_eqns AE lv).
+  edestruct exp_eval_same; try eapply H2; eauto; dcr.
+  inv X.
+  - congruence.
+  - econstructor. inv H5; congruence.
+Qed.
+
+Lemma cp_eqns_single AE x
+: cp_eqns AE {{ x }} [=] cp_eqn AE x.
+Proof.
+  unfold cp_eqns.
+  rewrite map_single; [| intuition].
+  erewrite fold_single; eauto.
   cset_tac; intuition.
-  rewrite <- H1. reflexivity.
+  eapply Equal_ST.
+  eapply union_m.
+  eapply transpose_union.
 Qed.
 
-Lemma entails_empty s
-: entails s ∅.
+Lemma cp_choose_moreDefined AE e lv
+: Exp.freeVars e ⊆ lv
+  -> moreDefined (cp_eqns AE lv) (cp_eqns AE lv) e (cp_choose_exp AE e).
 Proof.
-  hnf; intros. split; intros.
-  - hnf; intros. cset_tac; intuition.
-  - rewrite (incl_empty _ s). reflexivity.
+  unfold cp_choose_exp. case_eq (exp_eval AE e); intros.
+  - hnf; intros.
+      case_eq (Exp.exp_eval E e); intros.
+      * edestruct exp_eval_same; try eapply H2; eauto; dcr.
+        simpl. inv H7. econstructor. congruence.
+      * econstructor.
+  - reflexivity.
 Qed.
 
-
-Lemma cp_sound_eqn Lv Cp Es s al alv ang
-: let Gamma := (zip2Ann cp_eqns al alv (ann0 ∅)) in
-live_sound Lv s alv
--> cp_sound Cp s al alv
--> same_shape al alv
--> ssa s ang
--> eqn_sound Es s Gamma Gamma ang (cp_choose s al).
+Lemma cp_choose_moreDefinedArgs AE Y lv
+: list_union (List.map Exp.freeVars Y) ⊆ lv
+  -> moreDefinedArgs (cp_eqns AE lv) (cp_eqns AE lv) Y
+                    (List.map (cp_choose_exp AE) Y).
 Proof.
-  intros. subst Gamma.
-  general induction H0; invt live_sound; invt same_shape; invt ssa; simpl.
-  - econstructor.
-    eapply IHcp_sound; eauto. simpl in * |- *.
-    + rewrite zip2Ann_get; eauto.
-      destruct (in_or_not x (getAnn alv)); dcr.
-      * rewrite H7. rewrite cp_eqns_union. eapply entails_union; split.
-        {
-          rewrite <- (cp_eqns_agree H); eauto.
-          eapply entails_monotonic_add.
-          rewrite <- H13. reflexivity.
-        }
-        {
-          unfold cp_eqns. rewrite map_single; [| intuition].
-          rewrite (@fold_single _ _ _ Equal).
-          unfold cp_eqn at 2. case_eq (getAnn al x); intros.
-          destruct a. rewrite H8 in H1.
-          intros. rewrite union_comm, empty_neutral_union.
-          eapply exp_eval_entails; eauto.
-          rewrite empty_neutral_union.
-          eapply entails_empty.
-          rewrite empty_neutral_union.
-          eapply entails_empty.
-          eapply Equal_ST.
-          eapply union_m.
-          eapply transpose_union.
-        }
-
-      * rewrite H7. rewrite <- (cp_eqns_agree H); eauto.
-        eapply entails_monotonic_add.
-        rewrite <- H13. reflexivity.
-    + rewrite zip2Ann_get; eauto. admit.
-    +
-      unfold cp_choose_exp. case_eq (exp_eval Gamma e); intros.
-      case_eq a; intros; subst.
-      * hnf; intros.
-        case_eq (Exp.exp_eval E e); intros.
-        exploit exp_eval_same; try eapply H17; eauto.
-        simpl; eauto. inv X; econstructor; eauto.
+  intros. general induction Y; simpl.
+  - econstructor; eauto.
+  - hnf; intros; simpl.
+    unfold cp_choose_exp at 1.
+    case_eq (exp_eval AE a); intros.
+    + case_eq (Exp.exp_eval E a); intros.
+      * simpl.
+        exploit (IHY AE lv); eauto using get.
+        admit.
+        exploit X; eauto. inv X0; simpl.
         econstructor.
-      * reflexivity.
-      * reflexivity.
-    + unfold cp_choose_exp. case_eq (exp_eval Gamma e); intros; eauto.
-      case_eq a; intros; subst; simpl. eapply incl_empty. eassumption.
-  - admit.
-  - assert (exists a, get Es (counted l) a). admit.
-    destruct H4. destruct x as [[[[[Zb G] Γf] EqS] Γf'] EqS'].
+        edestruct exp_eval_same; try eapply H1; eauto using get; dcr.
+        edestruct exp_eval_same; try eapply H2; try eapply H4; eauto using get; dcr.
+        admit. admit.
+        inv H8; inv H9.
+        econstructor; eauto. congruence.
+      * simpl. econstructor.
+    + case_eq (Exp.exp_eval E a); intros; simpl; try econstructor; eauto.
+      erewrite exp_eval_onvLe; eauto. simpl.
+      exploit (IHY AE lv); eauto using get.
+      admit.
+      exploit X; eauto. inv X0; simpl.
+      * econstructor.
+      * econstructor; eauto.
+Qed.
+
+
+Lemma cp_choose_exp_freeVars AE e D
+: Exp.freeVars e ⊆ D
+  -> Exp.freeVars (cp_choose_exp AE e) ⊆ D.
+Proof.
+  intros.
+  unfold cp_choose_exp. case_eq (exp_eval AE e); intros; eauto using incl_empty.
+Qed.
+
+Lemma cp_choose_exp_live_sound_exp AE e lv
+:  Exp.freeVars e ⊆ lv
+   -> Exp.freeVars (cp_choose_exp AE e) ⊆ lv.
+Proof.
+  intros. unfold cp_choose_exp.
+  destruct (exp_eval AE e); intros; eauto.
+  simpl; eapply incl_empty.
+Qed.
+
+Lemma cp_choose_exp_eval_exp AE e v
+: exp_eval AE e = ⎣v ⎦
+  -> exp_eval AE (cp_choose_exp AE e) = ⎣v ⎦.
+Proof.
+  intros. unfold cp_choose_exp. rewrite H; eauto.
+Qed.
+
+Lemma update_with_list_lookup_in_list B E
+      (Z:list var) (Y:list B) z
+: length Z = length Y
+  -> z ∈ of_list Z
+  -> exists n y, get Z n z /\ get Y n y /\ E [Z <-- Y] z = y.
+Proof.
+  intros. eapply length_length_eq in H.
+  general induction H; simpl in *; isabsurd.
+  decide (z = x); subst.
+  exists 0, y; repeat split; eauto using get. lud. intuition.
+  edestruct (IHlength_eq E z) as [? [? ]]; eauto; dcr.
+  cset_tac; intuition. lud; intuition.
+  do 2 eexists; repeat split; eauto using get.
+Qed.
+
+
+Lemma subst_eqns_in gamma ϱ Gamma
+: gamma \In subst_eqns ϱ Gamma
+  -> exists γ', γ' ∈ Gamma /\ gamma = subst_eqn ϱ γ'.
+Proof.
+  intros. unfold subst_eqns in H.
+  eapply map_iff in H; eauto using subst_eqn_Proper.
+  destruct H; dcr. eexists x; split; eauto.
+  inv H1. hnf in *. subst.
+  destruct x; simpl. reflexivity.
+Qed.
+
+Lemma cp_eqns_in gamma AE lv
+: gamma \In cp_eqns AE lv
+  -> exists x, x ∈ lv /\ gamma ∈ cp_eqn AE x.
+Proof.
+  intros. unfold cp_eqns in H.
+  eapply incl_fold_union in H.
+  destruct H; isabsurd.
+  destruct H; dcr.
+  eapply map_iff in H0. destruct H0; dcr.
+  eexists x0; split; eauto. rewrite <- H2; eauto.
+  intuition.
+Qed.
+
+Lemma lookup_list_get (AE:onv aval) Z n x z
+: get (lookup_list AE Z) n x
+  -> get Z n z
+  -> x = AE z.
+Proof.
+  intros. general induction H0; simpl in *; inv H; eauto.
+Qed.
+
+Lemma cp_eqns_freeVars AE lv
+: eqns_freeVars (cp_eqns AE lv) ⊆ lv.
+Proof.
+  hnf; intros.
+  eapply incl_fold_union in H; destruct H; isabsurd.
+  destruct H; dcr.
+  eapply map_iff in H0; destruct H0; dcr; intuition.
+  eapply cp_eqns_in in H0. destruct H0; dcr.
+  eapply H2 in H1.
+  unfold cp_eqn in H3.
+  case_eq (AE x1); intros. rewrite H in H3. cset_tac.
+  hnf in H3. inv H3; hnf in *; subst. simpl in *.
+  cset_tac; intuition. rewrite <- H4. eauto.
+  rewrite H in H3. isabsurd.
+Qed.
+
+Lemma cp_sound_eqn AE Cp Es s (ang:ann (set var * set var))
+: let Gamma := (cp_eqns AE (fst (getAnn ang))) in
+cp_sound AE Cp s
+-> ssa s ang
+-> labelsDefined s Es
+-> (forall n a Z, get Es n a
+              -> get Cp n Z
+              -> snd a [=] cp_eqns AE (of_list Z)
+                /\ snd (fst (fst a)) [=] cp_eqns AE (of_list Z)
+                /\ fst (fst (fst (fst (fst a)))) = Z)
+-> eqn_sound Es s Gamma Gamma ang (cp_choose AE s).
+Proof.
+  intro. subst Gamma.
+  intros CP SSA LD LINV.
+  general induction CP; invt ssa; invt labelsDefined; simpl.
+  - econstructor.
+    eapply eqn_sound_entails_monotone; eauto.
+    + rewrite H7; simpl. rewrite cp_eqns_union.
+      eapply entails_union; split.
+      eapply entails_monotonic_add. reflexivity.
+
+      rewrite cp_eqns_single.
+      unfold cp_eqn. case_eq (AE x); intros; eauto using entails_empty.
+      eapply exp_eval_entails; eauto. congruence.
+    + rewrite H7; simpl.
+      rewrite cp_eqns_union. eapply entails_union; split.
+      eapply entails_monotonic_add. reflexivity.
+
+      rewrite cp_eqns_single.
+      unfold cp_eqn. case_eq (AE x); intros; eauto using entails_empty.
+      eapply exp_eval_entails; eauto.
+      eapply cp_choose_exp_live_sound_exp; eauto.
+      eapply cp_choose_exp_eval_exp; eauto.
+      congruence.
+    + eapply cp_choose_moreDefined; eauto.
+    + eapply cp_choose_exp_freeVars; eauto.
+  - econstructor; intros; eauto.
+    + eapply eqn_sound_entails_monotone; eauto.
+      eapply H0; eauto. intro.
+      edestruct H3; dcr.
+      eapply H16. hnf; simpl.
+      edestruct exp_eval_same; eauto; dcr.
+      rewrite H17. eauto.
+      * rewrite H12; eauto; reflexivity.
+      * rewrite H12; eauto; reflexivity.
+    + eapply eqn_sound_entails_monotone; eauto.
+      eapply H2; eauto. intro.
+      exfalso. edestruct H3; dcr.
+      eapply H16. hnf; simpl.
+      edestruct exp_eval_same; eauto; dcr.
+      rewrite H17. eauto.
+      * rewrite H13; eauto; reflexivity.
+      * rewrite H13; eauto; reflexivity.
+    + eapply cp_choose_moreDefined; eauto.
+  - destruct a as [[[[[Zb G] Γf] EqS] Γf'] EqS'].
+    exploit LINV; eauto; dcr; simpl in *. subst Zb.
     econstructor; eauto.
-    rewrite map_length; eauto.
+    + rewrite map_length; eauto.
+    + rewrite H5.
+      hnf. intros. hnf. intros.
+      edestruct subst_eqns_in as [γ' ?]; eauto; dcr; subst.
+      edestruct cp_eqns_in as [x ?]; eauto; dcr.
+      unfold cp_eqn in H12. case_eq (AE x); intros.
+      cset_tac. assert (γ' = (Var x, Con a)).
+      destruct γ'. rewrite H9 in H12. cset_tac. inv H12.
+      hnf in H16, H18. subst. eauto.
+      subst. unfold subst_eqn; simpl.
+      edestruct (update_with_list_lookup_in_list sid Z Y) as [? [? ]]; eauto; dcr.
 
-
-  - econstructor. admit.
-
-
-
-
-
-
+      edestruct PIR2_nth_2; eauto. eapply map_get_1; eauto.
+      dcr.
+      exploit lookup_list_get; eauto.
+      inversion H18; try congruence. subst.
+      edestruct exp_eval_same; eauto; dcr.
+      rewrite <- H4.
+      eapply incl_list_union. eapply map_get_1; eauto. reflexivity.
+      hnf; simpl. rewrite H19.
+      econstructor. inv H21. congruence.
+      exfalso. rewrite H9 in H12. isabsurd.
+    +
+      admit.
+    + eapply cp_choose_moreDefinedArgs; eauto.
+  - econstructor; eauto using cp_choose_moreDefined.
+  - eapply EqnLet with (Γ2:=cp_eqns AE D) (Γ2':=cp_eqns AE D) (EqS:=cp_eqns AE (of_list Z)) (EqS':=cp_eqns AE (of_list Z)).
+    + eapply eqn_sound_entails_monotone; eauto.
+      eapply IHCP1; eauto.
+      * eapply labelsDefined_any; try eapply H10; eauto.
+      * intros; simpl.
+        inv H; inv H0; simpl.
+        split. reflexivity. split. reflexivity. split; eauto.
+        eapply LINV; eauto.
+      * rewrite H6. simpl.
+        rewrite cp_eqns_union. reflexivity.
+      * rewrite H6. simpl.
+        rewrite cp_eqns_union. reflexivity.
+    + eapply eqn_sound_entails_monotone; eauto.
+      eapply IHCP2; eauto.
+      * eapply labelsDefined_any; try eapply H11; eauto.
+      * intros; simpl.
+        inv H; inv H0; simpl.
+        split. reflexivity. split. reflexivity. split; eauto.
+        eapply LINV; eauto.
+      * rewrite H9; reflexivity.
+      * rewrite H9; reflexivity.
+    + rewrite cp_eqns_freeVars. eapply incl_right.
+    + rewrite cp_eqns_freeVars. eapply incl_right.
+    + rewrite cp_eqns_freeVars. reflexivity.
+    + rewrite cp_eqns_freeVars. reflexivity.
+    + reflexivity.
+    + reflexivity.
 Qed.
 
 (*
